theories/TM/Hoare/HoareStdLib.v
@@ -1,7 +1,7 @@
 (** ** Hoare Rules for Machines from [Code/] *)
 
 From Undecidability Require Import ProgrammingTools.
-From Undecidability Require Import Hoare.HoareLogic Hoare.HoareCombinators Hoare.HoareRegister Hoare.HoareTactics.
+From Undecidability.TM.Hoare Require Import HoareLogic HoareCombinators HoareRegister HoareTactics HoareTacticsView.
 
 
 (** *** Copy.v *)
@@ -15,120 +15,118 @@ From Undecidability Require Import TM.Code.Copy.
 Definition CopyValue_sizefun {sigX X : Type} {cX : codable sigX X} (x : X) : Vector.t (nat->nat) 2 := [|id; CopyValue_size x|].
 
 Lemma CopyValue_SpecT_size (sig : finType) (sigX X : Type) (cX : codable sigX X) (I : Retract sigX sig) (x : X) (ss : Vector.t nat 2) :
-  TripleT (tspec (withSpace [|Contains _ x; Void|] ss))
-          (CopyValue_steps x) (CopyValue _)
-          (fun _ => tspec (withSpace [|Contains _ x; Contains _ x|] (appSize (CopyValue_sizefun x) ss))).
+  TripleT (tspec ([],withSpace [|Contains _ x; Void|] ss))
+          (CopyValue_steps x) (CopyValue sig)
+          (fun _ => tspec ([],withSpace [|Contains _ x; Contains _ x|] (appSize (CopyValue_sizefun x) ss))).
 Proof.
   eapply Realise_TripleT.
   - apply CopyValue_Realise.
   - apply CopyValue_Terminates.
-  - intros tin [] tout H HEnc. cbn in *. 
-    specialize (HEnc Fin0) as HEnc0; specialize (HEnc Fin1) as HEnc1. hnf. cbn in *. 
-    cbn in *; simpl_vector in *; cbn in *. unfold tspec_single in *. cbn in *.
-    modpon H. tspec_solve. 
-  - intros tin k HEnc. cbn in *.
+  - intros tin [] tout H HEnc. unfold withSpace in *|-. cbn in *. 
+    specialize (HEnc Fin0) as HEnc0; specialize (HEnc Fin1) as HEnc1. 
+    cbn in *; simpl_vector in *; cbn in *.
+    modpon H. tspec_solve.
+  - intros tin k HEnc. cbn in *. unfold withSpace in *.
     specialize (HEnc Fin0) as HEnc0; specialize (HEnc Fin1) as HEnc1.
     cbn in *; simpl_vector in *; cbn in *. eauto.
 Qed.
 
 Lemma CopyValue_SpecT (sig : finType) (sigX X : Type) (cX : codable sigX X) (I : Retract sigX sig) (x : X) :
-  TripleT (tspec (SpecVector [|Contains _ x; Void|])) (CopyValue_steps x) (CopyValue _) (fun _ => tspec (SpecVector [|Contains _ x; Contains _ x|])).
+  TripleT (tspec ([],[|Contains _ x; Void|])) (CopyValue_steps x) (CopyValue sig) (fun _ => tspec ([],[|Contains _ x; Contains _ x|])).
 Proof. eapply TripleT_RemoveSpace. cbn. intros s. apply CopyValue_SpecT_size. Qed.
 
 Lemma CopyValue_Spec_size (sig : finType) (sigX X : Type) (cX : codable sigX X) (I : Retract sigX sig) (x : X) (ss : Vector.t nat 2) :
-  Triple (tspec (withSpace (SpecVector [|Contains _ x; Void|]) ss))
-         (CopyValue _)
-         (fun _ => tspec (withSpace (SpecVector [|Contains _ x; Contains _ x|]) (appSize (CopyValue_sizefun x) ss))).
+  Triple (tspec (([], withSpace  [|Contains _ x; Void|] ss)))
+         (CopyValue sig)
+         (fun _ => tspec (([], withSpace  [|Contains _ x; Contains _ x|] (appSize (CopyValue_sizefun x) ss)))).
 Proof. eapply TripleT_Triple. apply CopyValue_SpecT_size. Qed.
 
 Lemma CopyValue_Spec (sig : finType) (sigX X : Type) (cX : codable sigX X) (I : Retract sigX sig) (x : X) :
-  Triple (tspec (SpecVector [|Contains _ x; Void|]))
-         (CopyValue _)
-         (fun _ => tspec (SpecVector [|Contains _ x; Contains _ x|])).
+  Triple (tspec ([],  [|Contains _ x; Void|]))
+         (CopyValue sig)
+         (fun _ => tspec ([],  [|Contains _ x; Contains _ x|])).
 Proof. eapply Triple_RemoveSpace. apply CopyValue_Spec_size. Qed.
 
 
 
 Lemma Reset_SpecT_space (sig : finType) (sigX X : Type) (cX : codable sigX X) (I : Retract sigX sig) (x : X) (ss : Vector.t nat 1) :
-  TripleT (tspec (withSpace (SpecVector [|Contains _ x|]) ss)) (Reset_steps x) (Reset _) (fun _ => tspec (withSpace (SpecVector [|Void|]) (appSize [|Reset_size x|] ss))).
+  TripleT (tspec ([], withSpace  [|Contains _ x |] ss)) (Reset_steps x) (Reset sig) (fun _ => tspec (([], withSpace  [|Void|] (appSize [|Reset_size x|] ss)))).
 Proof.
   eapply Realise_TripleT.
   - apply Reset_Realise.
   - apply Reset_Terminates.
-  - intros tin [] tout H HEnc. cbn in *.
+  - intros tin [] tout H HEnc. unfold withSpace in *. cbn in *.
     specialize (HEnc Fin0); cbn in *. simpl_vector in *; cbn in *.
     modpon H.
-    
-
     tspec_solve.
-  - intros tin k HEnc. cbn in *.
+  - intros tin k HEnc. unfold withSpace in *. cbn in *.
     specialize (HEnc Fin0). simpl_vector in *; cbn in *. eauto.
 Qed.
 
 Lemma Reset_SpecT (sig : finType) (sigX X : Type) (cX : codable sigX X) (I : Retract sigX sig) (x : X) :
-  TripleT (tspec (SpecVector [|Contains _ x|])) (Reset_steps x) (Reset _) (fun _ => tspec (SpecVector [|Void|])).
+  TripleT (tspec ([],  [|Contains _ x|])) (Reset_steps x) (Reset sig) (fun _ => tspec ([],  [|Void|])).
 Proof. eapply TripleT_RemoveSpace. apply Reset_SpecT_space. Qed.
 
 Lemma Reset_Spec_size (sig : finType) (sigX X : Type) (cX : codable sigX X) (I : Retract sigX sig) (x : X) ss :
-  Triple (tspec (withSpace (SpecVector [|Contains _ x|]) ss)) (Reset _) (fun _ => tspec (withSpace (SpecVector [|Void|]) (appSize [|Reset_size x|] ss))).
+  Triple (tspec (([], withSpace  [|Contains _ x |] ss))) (Reset sig) (fun _ => tspec (([], withSpace  [|Void|] (appSize [|Reset_size x|] ss)))).
 Proof. eapply TripleT_Triple. apply Reset_SpecT_space. Qed.
 
 Lemma Reset_Spec (sig : finType) (sigX X : Type) (cX : codable sigX X) (I : Retract sigX sig) (x : X) :
-  Triple (tspec (SpecVector [|Contains _ x|])) (Reset _) (fun _ => tspec (SpecVector [|Void|])).
+  Triple (tspec ([],  [|Contains _ x|])) (Reset sig) (fun _ => tspec ([],  [|Void|])).
 Proof. eapply TripleT_Triple. apply Reset_SpecT. Qed.
 
 
 Lemma ResetEmpty_SpecT_space (sig : finType) (sigX X : Type) (cX : codable sigX X) (I : Retract sigX sig) (x : X) (ss : Vector.t nat 1) :
   cX x = [] ->
-  TripleT (tspec (withSpace (SpecVector [|Contains _ x|]) ss)) (ResetEmpty_steps) (ResetEmpty _) (fun _ => tspec (withSpace (SpecVector [|Void|]) (appSize [|ResetEmpty_size|] ss))).
+  TripleT (tspec (([], withSpace  [|Contains _ x |] ss))) (ResetEmpty_steps) (ResetEmpty sig) (fun _ => tspec (([], withSpace  [|Void|] (appSize [|ResetEmpty_size|] ss)))).
 Proof.
   intros HEncEmpty. eapply RealiseIn_TripleT.
   - apply ResetEmpty_Sem.
-  - intros tin [] tout H HEnc. cbn in *.
+  - intros tin [] tout H HEnc. unfold withSpace in *. cbn in *.
     specialize (HEnc Fin0); cbn in *. simpl_vector in *; cbn in *.
     modpon H. tspec_solve.
 Qed.
 
 Lemma ResetEmpty_SpecT (sig : finType) (sigX X : Type) (cX : codable sigX X) (I : Retract sigX sig) (x : X) :
   cX x = [] ->
-  TripleT (tspec (SpecVector [|Contains _ x|])) (ResetEmpty_steps) (ResetEmpty _) (fun _ => tspec (SpecVector [|Void|])).
+  TripleT (tspec ([],  [|Contains _ x|])) (ResetEmpty_steps) (ResetEmpty sig) (fun _ => tspec ([],  [|Void|])).
 Proof. intros. eapply TripleT_RemoveSpace. intros. now apply ResetEmpty_SpecT_space. Qed.
 
 Lemma ResetEmpty_Spec_size (sig : finType) (sigX X : Type) (cX : codable sigX X) (I : Retract sigX sig) (x : X) ss :
   cX x = [] ->
-  Triple (tspec (withSpace (SpecVector [|Contains _ x|]) ss)) (ResetEmpty _) (fun _ => tspec (withSpace (SpecVector [|Void|]) (appSize [|ResetEmpty_size|] ss))).
+  Triple (tspec (([], withSpace  [|Contains _ x |] ss))) (ResetEmpty sig) (fun _ => tspec (([], withSpace  [|Void|] (appSize [|ResetEmpty_size|] ss)))).
 Proof. intros. eapply TripleT_Triple. now apply ResetEmpty_SpecT_space. Qed.
 
 Lemma ResetEmpty_Spec (sig : finType) (sigX X : Type) (cX : codable sigX X) (I : Retract sigX sig) (x : X) :
   cX x = [] ->
-  Triple (tspec (SpecVector [|Contains _ x|])) (ResetEmpty _) (fun _ => tspec (SpecVector [|Void|])).
+  Triple (tspec ([],  [|Contains _ x|])) (ResetEmpty sig) (fun _ => tspec ([],  [|Void|])).
 Proof. intros. eapply TripleT_Triple. now apply ResetEmpty_SpecT. Qed.
 
 
 Lemma ResetEmpty1_SpecT_space (sig : finType) (sigX X : Type) (cX : codable sigX X) (I : Retract sigX sig) (x : X) (ss : Vector.t nat 1) :
   size cX x = 1 ->
-  TripleT (tspec (withSpace (SpecVector [|Contains _ x|]) ss)) (ResetEmpty1_steps) (ResetEmpty1 _) (fun _ => tspec (withSpace (SpecVector [|Void|]) (appSize [|ResetEmpty1_size|] ss))).
+  TripleT (tspec (([], withSpace  [|Contains _ x |] ss))) (ResetEmpty1_steps) (ResetEmpty1 sig) (fun _ => tspec (([], withSpace  [|Void|] (appSize [|ResetEmpty1_size|] ss)))).
 Proof.
   intros HEncEmpty. eapply RealiseIn_TripleT.
   - apply ResetEmpty1_Sem.
-  - intros tin [] tout H HEnc. cbn in *.
+  - intros tin [] tout H HEnc. cbn in *. unfold withSpace in *.
     specialize (HEnc Fin0); cbn in *. simpl_vector in *; cbn in *.
     modpon H. tspec_solve.
 Qed.
 
 Lemma ResetEmpty1_SpecT (sig : finType) (sigX X : Type) (cX : codable sigX X) (I : Retract sigX sig) (x : X) :
   size cX x = 1 ->
-  TripleT (tspec (SpecVector [|Contains _ x|])) (ResetEmpty1_steps) (ResetEmpty1 _) (fun _ => tspec (SpecVector [|Void|])).
+  TripleT (tspec ([],  [|Contains _ x|])) (ResetEmpty1_steps) (ResetEmpty1 sig) (fun _ => tspec ([],  [|Void|])).
 Proof. intros. eapply TripleT_RemoveSpace. intros. now apply ResetEmpty1_SpecT_space. Qed.
 
 Lemma ResetEmpty1_Spec_size (sig : finType) (sigX X : Type) (cX : codable sigX X) (I : Retract sigX sig) (x : X) ss :
   size cX x = 1 ->
-  Triple (tspec (withSpace (SpecVector [|Contains _ x|]) ss)) (ResetEmpty1 _) (fun _ => tspec (withSpace (SpecVector [|Void|]) (appSize [|ResetEmpty1_size|] ss))).
+  Triple (tspec (([], withSpace  [|Contains _ x |] ss))) (ResetEmpty1 sig) (fun _ => tspec (([], withSpace  [|Void|] (appSize [|ResetEmpty1_size|] ss)))).
 Proof. intros. eapply TripleT_Triple. now apply ResetEmpty1_SpecT_space. Qed.
 
 Lemma ResetEmpty1_Spec (sig : finType) (sigX X : Type) (cX : codable sigX X) (I : Retract sigX sig) (x : X) :
   size cX x = 1 ->
-  Triple (tspec (SpecVector [|Contains _ x|])) (ResetEmpty1 _) (fun _ => tspec (SpecVector [|Void|])).
+  Triple (tspec ([],  [|Contains _ x|])) (ResetEmpty1 sig) (fun _ => tspec ([],  [|Void|])).
 Proof. intros. eapply TripleT_Triple. now apply ResetEmpty1_SpecT. Qed.
 
 
@@ -139,9 +137,9 @@ Definition MoveValue_size {X Y sigX sigY : Type} {cX : codable sigX X} {cY : cod
 
 Lemma MoveValue_SpecT_size (sig : finType) (sigX sigY X Y : Type)
       (cX : codable sigX X) (cY : codable sigY Y) (I1 : Retract sigX sig) (I2 : Retract sigY sig) (x : X) (y : Y) (ss : Vector.t nat 2) :
-  TripleT (tspec (withSpace (SpecVector [|Contains _ x; Contains _ y|]) ss)) (MoveValue_steps x y) (MoveValue _)
-          (fun _ => tspec (withSpace (SpecVector [|Void; Contains _ x|]) (appSize (MoveValue_size x y) ss))).
-Proof.
+  TripleT (tspec (([], withSpace  [|Contains _ x; Contains _ y |] ss))) (MoveValue_steps x y) (MoveValue sig)
+          (fun _ => tspec (([], withSpace  [|Void; Contains _ x|] (appSize (MoveValue_size x y) ss)))).
+Proof. unfold withSpace.
   eapply Realise_TripleT.
   - apply MoveValue_Realise with (X := X) (Y := Y).
   - apply MoveValue_Terminates with (X := X) (Y := Y).
@@ -154,26 +152,26 @@ Qed.
 
 Lemma MoveValue_SpecT (sig : finType) (sigX sigY X Y : Type)
       (cX : codable sigX X) (cY : codable sigY Y) (I1 : Retract sigX sig) (I2 : Retract sigY sig) (x : X) (y : Y) :
-  TripleT (tspec (SpecVector [|Contains _ x; Contains _ y|])) (MoveValue_steps x y) (MoveValue _) (fun _ => tspec (SpecVector [|Void; Contains _ x|])).
+  TripleT (tspec ([],  [|Contains _ x; Contains _ y|])) (MoveValue_steps x y) (MoveValue sig) (fun _ => tspec ([],  [|Void; Contains _ x|])).
 Proof. eapply TripleT_RemoveSpace. apply MoveValue_SpecT_size. Qed.
 
 Lemma MoveValue_Spec_size (sig : finType) (sigX sigY X Y : Type)
       (cX : codable sigX X) (cY : codable sigY Y) (I1 : Retract sigX sig) (I2 : Retract sigY sig) (x : X) (y : Y) (ss : Vector.t nat 2) :
-  Triple (tspec (withSpace (SpecVector [|Contains _ x; Contains _ y|]) ss)) (MoveValue _)
-         (fun _ => tspec (withSpace (SpecVector [|Void; Contains _ x|]) (appSize (MoveValue_size x y) ss))).
+  Triple (tspec (([], withSpace  [|Contains _ x; Contains _ y |] ss))) (MoveValue sig)
+         (fun _ => tspec (([], withSpace  [|Void; Contains _ x|] (appSize (MoveValue_size x y) ss)))).
 Proof. eapply TripleT_Triple. apply MoveValue_SpecT_size. Qed.
 
 Lemma MoveValue_Spec (sig : finType) (sigX sigY X Y : Type)
       (cX : codable sigX X) (cY : codable sigY Y) (I1 : Retract sigX sig) (I2 : Retract sigY sig) (x : X) (y : Y) :
-  Triple (tspec (SpecVector [|Contains _ x; Contains _ y|])) (MoveValue _) (fun _ => tspec (SpecVector [|Void; Contains _ x|])).
+  Triple (tspec ([],  [|Contains _ x; Contains _ y|])) (MoveValue sig) (fun _ => tspec ([],  [|Void; Contains _ x|])).
 Proof. eapply TripleT_Triple. apply MoveValue_SpecT. Qed.
 
 
 Lemma Translate_SpecT_size (sig : finType) (sigX X : Type)
       (cX : codable sigX X) (I1 I2 : Retract sigX sig) (x : X) (ss : Vector.t nat 1) :
-  TripleT (tspec (withSpace (SpecVector [|Contains I1 x|]) ss)) (Translate_steps x) (Translate I1 I2)
-          (fun _ => tspec (withSpace (SpecVector [|Contains I2 x|]) (appSize [|id|] ss))).
-Proof.
+  TripleT (tspec (([], withSpace  [|Contains I1 x |] ss))) (Translate_steps x) (Translate I1 I2)
+          (fun _ => tspec (([], withSpace  [|Contains I2 x|] (appSize [|id|] ss)))).
+Proof. unfold withSpace.
   eapply Realise_TripleT.
   - apply Translate_Realise with (X := X).
   - apply Translate_Terminates with (X := X).
@@ -186,20 +184,20 @@ Qed.
 
 Lemma Translate_SpecT (sig : finType) (sigX X : Type)
       (cX : codable sigX X) (I1 I2 : Retract sigX sig) (x : X) :
-  TripleT (tspec (SpecVector [|Contains I1 x|])) (Translate_steps x) (Translate I1 I2)
-          (fun _ => tspec (SpecVector [|Contains I2 x|])).
+  TripleT (tspec ([],  [|Contains I1 x|])) (Translate_steps x) (Translate I1 I2)
+          (fun _ => tspec ([],  [|Contains I2 x|])).
 Proof. eapply TripleT_RemoveSpace. apply Translate_SpecT_size. Qed.
 
 Lemma Translate_Spec_size (sig : finType) (sigX X : Type)
       (cX : codable sigX X) (I1 I2 : Retract sigX sig) (x : X) (ss : Vector.t nat 1) :
-  Triple (tspec (withSpace (SpecVector [|Contains I1 x|]) ss)) (Translate I1 I2)
-         (fun _ => tspec (withSpace (SpecVector [|Contains I2 x|]) (appSize [|id|] ss))).
+  Triple (tspec (([], withSpace  [|Contains I1 x |] ss))) (Translate I1 I2)
+         (fun _ => tspec (([], withSpace  [|Contains I2 x|] (appSize [|id|] ss)))).
 Proof. eapply TripleT_Triple. apply Translate_SpecT_size. Qed.
 
 Lemma Translate_Spec (sig : finType) (sigX X : Type)
       (cX : codable sigX X) (I1 I2 : Retract sigX sig) (x : X) :
-  Triple (tspec (SpecVector [|Contains I1 x|])) (Translate I1 I2)
-         (fun _ => tspec (SpecVector [|Contains I2 x|])).
+  Triple (tspec ([],  [|Contains I1 x|])) (Translate I1 I2)
+         (fun _ => tspec ([],  [|Contains I2 x|])).
 Proof. eapply TripleT_Triple. apply Translate_SpecT. Qed.
 
 
@@ -221,10 +219,10 @@ Section CompareValues.
   Hypothesis (HInj : forall x y, cX x = cX y -> x = y).
 
   Lemma CompareValue_SpecT_size (x y : X) (ss : Vector.t nat 2) :
-    TripleT (tspec (withSpace (SpecVector [|Contains _ x; Contains _ y|]) ss))
+    TripleT (tspec (([], withSpace  [|Contains _ x; Contains _ y |] ss)))
             (CompareValues_steps x y) (CompareValues sigX)
-            (fun yout => tspec (withSpace ([if yout then x=y else x<>y],[|Contains _ x; Contains _ y|]) (appSize [|id; id|] ss))).
-  Proof.
+            (fun yout => tspec ([if yout then x=y else x<>y],withSpace [|Contains _ x; Contains _ y|] (appSize [|id; id|] ss))).
+  Proof. unfold withSpace.
     eapply Realise_TripleT.
     - now apply CompareValues_Realise.
     - now apply CompareValues_TerminatesIn.
@@ -239,19 +237,19 @@ Section CompareValues.
   Qed.
 
   Lemma CompareValue_SpecT (x y : X) :
-    TripleT (tspec (SpecVector [|Contains _ x; Contains _ y|]))
+    TripleT (tspec ([],  [|Contains _ x; Contains _ y|]))
             (CompareValues_steps x y) (CompareValues sigX)
             (fun yout => tspec ([if yout then x=y else x<>y],[|Contains _ x; Contains _ y|])).
   Proof. eapply TripleT_RemoveSpace. cbn. intros s. apply CompareValue_SpecT_size. Qed.
 
   Lemma CompareValue_Spec_size (x y : X) (ss : Vector.t nat 2) :
-    Triple (tspec (withSpace (SpecVector [|Contains _ x; Contains _ y|]) ss))
+    Triple (tspec (([], withSpace  [|Contains _ x; Contains _ y |] ss)))
            (CompareValues sigX)
-           (fun yout => tspec (withSpace ([if yout then x=y else x<>y],[|Contains _ x; Contains _ y|]) (appSize [|id; id|] ss))).
+           (fun yout => tspec ([if yout then x=y else x<>y],withSpace [|Contains _ x; Contains _ y|] (appSize [|id; id|] ss))).
   Proof. eapply TripleT_Triple. apply CompareValue_SpecT_size. Qed.
 
   Lemma CompareValue_Spec (x y : X) :
-    Triple (tspec (SpecVector [|Contains _ x; Contains _ y|]))
+    Triple (tspec ([],  [|Contains _ x; Contains _ y|]))
            (CompareValues sigX)
            (fun yout => tspec ([if yout then x=y else x<>y],[|Contains _ x; Contains _ y|])).
   Proof. eapply Triple_RemoveSpace. apply CompareValue_Spec_size. Qed.
@@ -267,8 +265,8 @@ From Undecidability Require Import TM.Code.CaseNat.
 (** Here, we only need to register the strongest version; the automation takes care of everything. *)
 
 Lemma Constr_O_SpecT_size (ss : Vector.t nat 1) :
-  TripleT (tspec (withSpace (SpecVector [|Void|]) ss)) Constr_O_steps Constr_O (fun _ => tspec (withSpace (SpecVector [|Contains _ 0|]) (appSize [|Constr_O_size|] ss))).
-Proof.
+  TripleT (tspec (([], withSpace  [|Void |] ss))) Constr_O_steps Constr_O (fun _ => tspec (([], withSpace  [|Contains _ 0|] (appSize [|Constr_O_size|] ss)))).
+Proof.  unfold withSpace.
   eapply RealiseIn_TripleT.
   - apply Constr_O_Sem.
   - intros tin [] tout H1 H2. cbn in *. specialize (H2 Fin0). simpl_vector in *; cbn in *. modpon H1. tspec_solve.
@@ -276,9 +274,9 @@ Qed.
 
 Lemma Constr_S_SpecT_size :
   forall (y : nat) ss,
-    TripleT (tspec (withSpace (SpecVector [|Contains _ y|]) ss)) Constr_S_steps Constr_S
-            (fun _ => tspec (withSpace (SpecVector [|Contains _ (S y)|]) (appSize [|S|] ss))).
-Proof.
+    TripleT (tspec (([], withSpace  [|Contains _ y |] ss))) Constr_S_steps Constr_S
+            (fun _ => tspec (([], withSpace  [|Contains _ (S y)|] (appSize [|S|] ss)))).
+Proof.  unfold withSpace.
   intros y ss.
   eapply RealiseIn_TripleT.
   - apply Constr_S_Sem.
@@ -294,14 +292,14 @@ Definition CaseNat_size (n : nat) : Vector.t (nat->nat) 1 :=
 
 Lemma CaseNat_SpecT_size (y : nat) (ss : Vector.t nat 1) :
   TripleT
-    (tspec (withSpace (SpecVector [|Contains _ y|]) ss))
+    (tspec (([], withSpace  [|Contains _ y |] ss)))
     CaseNat_steps
     CaseNat
     (fun yout =>
        tspec
-         (withSpace ([if yout then y <> 0 else y = 0],[|Contains _ (pred y)|])
+         ([if yout then y <> 0 else y = 0],withSpace ([|Contains _ (pred y)|])
             (appSize (CaseNat_size y) ss))).
-Proof.
+Proof.  unfold withSpace.
   eapply RealiseIn_TripleT.
   - apply CaseNat_Sem.
   - intros tin yout tout H HEnc. specialize (HEnc Fin0). simpl_vector in *; cbn in *. modpon H.
@@ -331,15 +329,15 @@ Definition CaseBool_size (_ : bool) : Vector.t (nat->nat) 1 :=
 
 Lemma CaseBool_SpecT_size (b : bool) (ss : Vector.t nat 1) :
   TripleT
-    (tspec (withSpace (SpecVector [|Contains _ b|]) ss))
+    (tspec (([], withSpace  [|Contains _ b |] ss)))
     CaseBool_steps
     CaseBool
     (fun yout =>
        tspec
-         (withSpace
-            ([yout = b],[|Void|])
+         ([yout = b],withSpace
+            ([|Void|])
             (appSize (CaseBool_size b) ss))). 
-Proof.
+Proof.  unfold withSpace.
   eapply RealiseIn_TripleT.
   - apply CaseBool_Sem.
   - intros tin yout tout H HEnc. specialize (HEnc Fin0). simpl_vector in *; cbn in *. modpon H.
@@ -363,9 +361,9 @@ Section CaseSum.
 
   Lemma Constr_inl_SpecT_size (x : X) (ss : Vector.t nat 1) :
     TripleT
-      (tspec (withSpace (SpecVector [|Contains _ x|]) ss)) Constr_inl_steps (Constr_inl sigX sigY)
-      (fun _ => tspec (withSpace (SpecVector [|Contains _ (inl x)|]) (appSize [|pred|] ss))).
-  Proof.
+      (tspec (([], withSpace  [|Contains _ x |] ss))) Constr_inl_steps (Constr_inl sigX sigY)
+      (fun _ => tspec (([], withSpace  [|Contains _ (inl x)|] (appSize [|pred|] ss)))).
+  Proof. unfold withSpace.
     eapply RealiseIn_TripleT.
     - apply Constr_inl_Sem.
     - intros tin [] tout H HEnc. cbn in *.
@@ -374,9 +372,9 @@ Section CaseSum.
 
   Lemma Constr_inr_SpecT_size (y : Y) (ss : Vector.t nat 1) :
     TripleT
-      (tspec (withSpace (SpecVector [|Contains _ y|]) ss)) Constr_inr_steps (Constr_inr sigX sigY)
-      (fun _ => tspec (withSpace (SpecVector [|Contains _ (inr y)|]) (appSize [|pred|] ss))).
-  Proof.
+      (tspec (([], withSpace  [|Contains _ y |] ss))) Constr_inr_steps (Constr_inr sigX sigY)
+      (fun _ => tspec (([], withSpace  [|Contains _ (inr y)|] (appSize [|pred|] ss)))).
+  Proof. unfold withSpace.
     eapply RealiseIn_TripleT.
     - apply Constr_inr_Sem.
     - intros tin [] tout H HEnc. cbn in *.
@@ -385,12 +383,11 @@ Section CaseSum.
 
   Lemma CaseSum_SpecT_size (s : X+Y) (ss : Vector.t nat 1) :
     TripleT
-      (tspec (withSpace (SpecVector [|Contains _ s|]) ss)) (CaseSum_steps) (CaseSum sigX sigY)
-      (fun yout => tspec (withSpace
-                         ([yout = if s then true else false],
-                          match s with inl x => [|Contains _ x|] | inr y =>  [|Contains _ y|] end)
+      (tspec (([], withSpace  [|Contains _ s |] ss))) (CaseSum_steps) (CaseSum sigX sigY)
+      (fun yout => tspec ([yout = if s then true else false],withSpace
+                         (match s with inl x => [|Contains _ x|] | inr y =>  [|Contains _ y|] end)
                          (appSize [|S|] ss))).
-  Proof.
+  Proof. unfold withSpace.
     eapply RealiseIn_TripleT.
     - apply CaseSum_Sem.
     - intros tin yout tout H HEnc. cbn in *.
@@ -407,9 +404,9 @@ Section CaseOpton.
 
   Lemma Constr_Some_SpecT_size (x : X) (ss : Vector.t nat 1) :
     TripleT
-      (tspec (withSpace (SpecVector [|Contains _ x|]) ss)) Constr_Some_steps (Constr_Some sigX)
-      (fun _ => tspec (withSpace (SpecVector [|Contains _ (Some x)|]) (appSize [|pred|] ss))).
-  Proof.
+      (tspec (([], withSpace  [|Contains _ x |] ss))) Constr_Some_steps (Constr_Some sigX)
+      (fun _ => tspec (([], withSpace  [|Contains _ (Some x)|] (appSize [|pred|] ss)))).
+  Proof. unfold withSpace.
     eapply RealiseIn_TripleT.
     - apply Constr_Some_Sem.
     - intros tin [] tout H HEnc. cbn in *.
@@ -418,9 +415,9 @@ Section CaseOpton.
 
   Lemma Constr_None_SpecT_size (ss : Vector.t nat 1) :
     TripleT
-      (tspec (withSpace (SpecVector [|Void|]) ss)) Constr_None_steps (Constr_None sigX)
-      (fun _ => tspec (withSpace (SpecVector [|Contains _ None|]) (appSize [|pred|] ss))).
-  Proof.
+      (tspec (([], withSpace  [|Void |] ss))) Constr_None_steps (Constr_None sigX)
+      (fun _ => tspec (([], withSpace  [|Contains _ None|] (appSize [|pred|] ss)))).
+  Proof. unfold withSpace.
     eapply RealiseIn_TripleT.
     - apply Constr_None_Sem.
     - intros tin [] tout H HEnc. cbn in *.
@@ -435,15 +432,14 @@ Section CaseOpton.
 
   Lemma CaseOption_SpecT_size (o : option X) (ss : Vector.t nat 1) :
     TripleT
-      (tspec (withSpace (SpecVector [|Contains _ o|]) ss)) (CaseOption_steps) (CaseOption sigX)
-      (fun yout => tspec (withSpace
-                         ([yout = match o with None => false | _ => true end ],
-                          match o with
+      (tspec (([], withSpace  [|Contains _ o |] ss))) (CaseOption_steps) (CaseOption sigX)
+      (fun yout => tspec ([yout = match o with None => false | _ => true end ],withSpace
+                         (match o with
                           |  Some x => [|Contains _ x|]
                           |  None  => [|Void|]
                           end)
                          (appSize (CaseOption_size o) ss))).
-  Proof.
+  Proof. unfold withSpace.
     eapply RealiseIn_TripleT.
     - apply CaseOption_Sem.
     - intros tin yout tout H HEnc. cbn in *.
@@ -481,9 +477,9 @@ Section CaseList.
 
   Lemma Constr_cons_SpecT_size (x : X) (xs : list X) (ss : Vector.t nat 2) :
     TripleT
-      (tspec (withSpace (SpecVector [|Contains _ xs; Contains _ x|]) ss)) (Constr_cons_steps x) (Constr_cons sigX)
-      (fun _ => tspec (withSpace (SpecVector [|Contains _ (x::xs); Contains _ x|]) (appSize (Constr_cons_sizefun x) ss))).
-  Proof.
+      (tspec (([], withSpace  [|Contains _ xs; Contains _ x |] ss))) (Constr_cons_steps x) (Constr_cons sigX)
+      (fun _ => tspec (([], withSpace  [|Contains _ (x::xs); Contains _ x|] (appSize (Constr_cons_sizefun x) ss)))).
+  Proof. unfold withSpace.
     eapply Realise_TripleT.
     - apply Constr_cons_Realise.
     - apply Constr_cons_Terminates.
@@ -497,9 +493,9 @@ Section CaseList.
 
   Lemma Constr_nil_SpecT_size (ss : Vector.t nat 1) :
     TripleT
-      (tspec (withSpace (SpecVector [|Void|]) ss)) Constr_nil_steps (Constr_nil sigX)
-      (fun _ => tspec (withSpace (SpecVector [|Contains _ nil|]) (appSize [|pred|] ss))).
-  Proof.
+      (tspec (([], withSpace  [|Void |] ss))) Constr_nil_steps (Constr_nil sigX)
+      (fun _ => tspec (([], withSpace  [|Contains _ nil|] (appSize [|pred|] ss)))).
+  Proof. unfold withSpace.
     eapply RealiseIn_TripleT.
     - apply Constr_nil_Sem.
     - intros tin [] tout H HEnc. cbn in *.
@@ -514,14 +510,14 @@ Section CaseList.
 
   Lemma CaseList_SpecT_size (xs : list X) (ss : Vector.t nat 2) :
     TripleT
-      (tspec (withSpace (SpecVector [|Contains _ xs; Void|]) ss)) (CaseList_steps xs) (CaseList sigX)
-      (fun yout => tspec (withSpace
-                         ([yout = match xs with [] => false | _ => true end] ,match xs with
+      (tspec (([], withSpace  [|Contains _ xs; Void |] ss))) (CaseList_steps xs) (CaseList sigX)
+      (fun yout => tspec ([yout = match xs with [] => false | _ => true end],withSpace
+                         (match xs with
                           |   x::xs' => [|Contains _ xs'; Contains _ x|]
                           |    nil => [|Contains _ xs; Void|]
                           end)
                          (appSize (CaseList_size xs) ss))).
-  Proof.
+  Proof. unfold withSpace.
     eapply Realise_TripleT.
     - apply CaseList_Realise.
     - apply CaseList_Terminates.
@@ -560,12 +556,13 @@ Section CasePair.
   Definition Constr_pair_sizefun (x : X) : Vector.t (nat->nat) 2 :=
     [|id; Constr_pair_size x|].
 
+  
   Lemma Constr_pair_SpecT_size (x : X) (y : Y) (ss : Vector.t nat 2) :
-    TripleT (tspec (withSpace (SpecVector [|Contains _ x; Contains _ y|]) ss))
+    TripleT (tspec (([], withSpace  [|Contains _ x; Contains _ y |] ss)))
             (Constr_pair_steps x) (Constr_pair sigX sigY)
-            (fun _ => tspec (withSpace (SpecVector [|Contains _ x; Contains _ (x,y)|])
-                                    (appSize (Constr_pair_sizefun x) ss))).
-  Proof.
+            (fun _ => tspec (([], withSpace  [|Contains _ x; Contains _ (x,y)|]
+                                    (appSize (Constr_pair_sizefun x) ss)))).
+  Proof. unfold withSpace.
     eapply Realise_TripleT.
     - apply Constr_pair_Realise.
     - apply Constr_pair_Terminates.
@@ -581,11 +578,11 @@ Section CasePair.
     [| CasePair_size0 (fst p); CasePair_size1 (fst p) |].
 
   Lemma CasePair_SpecT_size (p : X*Y) (ss : Vector.t nat 2) :
-    TripleT (tspec (withSpace (SpecVector [|Contains _ p; Void|]) ss))
+    TripleT (tspec (([], withSpace  [|Contains _ p; Void |] ss)))
             (CasePair_steps (fst p)) (CasePair sigX sigY)
-            (fun _ => tspec (withSpace (SpecVector [|Contains _ (snd p); Contains _ (fst p)|])
-                                    (appSize (CasePair_size p) ss))).
-  Proof.
+            (fun _ => tspec (([], withSpace  [|Contains _ (snd p); Contains _ (fst p)|]
+                                    (appSize (CasePair_size p) ss)))).
+  Proof. unfold withSpace.
     eapply Realise_TripleT.
     - apply CasePair_Realise.
     - apply CasePair_Terminates.
@@ -602,8 +599,8 @@ End CasePair.
 
 Ltac hstep_Pair :=
   match goal with
-  | [ |- TripleT ?P ?k (Constr_pair _ _) ?Q ] => eapply Constr_pair_SpecT_size
-  | [ |- TripleT ?P ?k (CasePair    _ _) ?Q ] => eapply CasePair_SpecT_size
+  | [ |- TripleT ?P ?k (Constr_pair _ _) ?Q ] => eapply (Constr_pair_SpecT_size _ _ _ _ _)
+  | [ |- TripleT ?P ?k (CasePair    _ _) ?Q ] => eapply (CasePair_SpecT_size _ _ _ _)
   end.
 
 Smpl Add hstep_Pair : hstep_smpl.
@@ -628,14 +625,14 @@ Section CaseFin.
   Definition CaseFin_size : Vector.t (nat->nat) 1 := [|S>>S|].
 
   Lemma CaseFin_SpecT_size (x : sig) (ss : Vector.t nat 1) :
-    TripleT (tspec (withSpace (SpecVector [|Contains _ x|]) ss))
+    TripleT (tspec (([], withSpace  [|Contains _ x |] ss)))
             (CaseFin_steps) (CaseFin sig)
-            (fun yout tout => tspec (withSpace (SpecVector [|Void|]) (appSize CaseFin_size ss)) tout /\ yout = x).
-  Proof.
+            (fun yout => tspec ([yout = x], withSpace  [|Void|] (appSize CaseFin_size ss))).
+  Proof. unfold withSpace in *.
     eapply RealiseIn_TripleT.
     - apply CaseFin_Sem.
     - intros tin yout tout H HEnc. cbn in *.
-      specialize (HEnc Fin0). simpl_vector in *; cbn in *. modpon H. split; auto. tspec_solve.
+      specialize (HEnc Fin0). simpl_vector in *; cbn in *. modpon H. tspec_solve. easy.
   Qed.
 
 End CaseFin.
@@ -664,10 +661,10 @@ Section WriteValue.
   Definition WriteValue_sizefun (x : X) : Vector.t (nat->nat) 1 := [| WriteValue_size x |].
   
   Lemma WriteValue_SpecT_size (x : X) (ss : Vector.t nat 1) :
-    TripleT (tspec (withSpace (SpecVector [|Void|]) ss))
+    TripleT (tspec (([], withSpace  [|Void |] ss)))
             (WriteValue_steps (size _ x)) (WriteValue (encode x))
-            (fun _ => tspec (withSpace (SpecVector [|Contains _ x|]) (appSize (WriteValue_sizefun x) ss))).
-  Proof.
+            (fun _ => tspec (([], withSpace  [|Contains _ x|] (appSize (WriteValue_sizefun x) ss)))).
+  Proof. unfold withSpace.
     eapply RealiseIn_TripleT.
     - apply WriteValue_Sem.
     - intros tin yout tout H HEnc. cbn in *.
